## Expanding Binomial Products
- $(k+4)$ and $(k-6)$ are called **binomial expressions** because each expression has exactly two terms (binomial = '2 terms').
- $(k+4)(k-6) is called a **binomial product** because it is a product(multiplication) of two binomial expressions
- When expanding a binomial product algebraically, each term in the first binomial is multiplied by each term in the second binomial to give **four terms**, which are collected and simplified. 
- $(k+4)(k=6) = k(k-6) + 4(k-6)$
- = $k^2 - 6k + 4k - 24$
- = $k^2 - 2k - 24$
- One way of remembering which pair of terms multiply together is the FOIL method. 
- F - First
- O - Outside
- I - Inside
- L - Last
#School 
